theories/IntersectionTypes/Reductions/SSTS01_to_CD_INH.v
@@ -1,0 +1,676 @@
+(*
+reduction from SSTS01 to intersection type inhabitation
+*)
+
+Require Import Undecidability.IntersectionTypes.CD Undecidability.IntersectionTypes.Util.CD_facts.
+
+Require Import Undecidability.StringRewriting.SSTS.
+
+Require Import Relations List PeanoNat Lia.
+Import ListNotations.
+
+Import CD (var, app, lam).
+
+Require Import ssreflect ssrbool ssrfun.
+
+Lemma map_nth_seq {X : Type} (l : list X) d : 
+  map (fun i => nth i l d) (seq 0 (length l)) = l.
+Proof.
+  elim: l; first done.
+  move=> ? ? IH /=. by rewrite -seq_shift map_map IH.
+Qed.
+
+(* transforms a goal (A -> B) -> C into goals A and B -> C *)
+Lemma unnest : forall (A B C : Type), A -> (B -> C) -> (A -> B) -> C.
+Proof. auto. Qed.
+
+Lemma Forall_In_impl {X : Type} {P Q : X -> Prop} {l : list X} :
+  (forall x, In x l -> P x -> Q x) -> Forall P l -> Forall Q l.
+Proof. move=> ? /Forall_forall ?. apply /Forall_forall. by auto with nocore. Qed.
+
+Lemma step_spec (rs : Ssts) a b a' b' i v : In ((a, b), (a', b')) rs ->
+  nth_error v i = Some a -> nth_error v (S i) = Some b ->
+  step rs v (map (fun j => if Nat.eqb j i then a' else if Nat.eqb j (S i) then b' else nth j v 0) (seq 0 (length v))).
+Proof.
+  move=> /step_intro H. elim: i v.
+  { move=> [|? [|? v]] /=; [done|done|].
+    move=> [->] [->]. have := H [] v.
+    by rewrite -!seq_shift !map_map /= map_nth_seq. }
+  move=> i IH [|? v] /=; first done.
+  move=> /IH /[apply]. rewrite -!seq_shift !map_map /=.
+  move: (map _ _) => ? [] > /step_intro H'.
+  by apply: (H' (_ :: _) _).
+Qed.
+
+Lemma step_length_eq (rs : Ssts) v w : step rs v w -> length v = length w.
+Proof. case => > _. by rewrite !app_length. Qed.
+
+Section Argument.
+
+Notation bullet := (atom 0).
+Notation star := (atom 1).
+(*indicates second symbol*)
+Notation hash := (atom 2).
+(*indicates first symbol*)
+Notation dollar := (atom 3).
+(*indicates very first split, used once*)
+Notation triangle := (atom 4).
+Notation isl := (atom 5).
+Notation isr := (atom 6).
+
+(*encodes elements of the alphabet including 0 and 1*)
+Definition symbol (a : nat) := atom (7 + a).
+
+Definition arr' phi t :=
+  match phi with
+  | [] => t
+  | s::phi => arr s phi t
+  end.
+
+#[local] Arguments arr' /.
+
+Definition mk_ty phi :=
+  match phi with
+  | [] => (atom 0, [])
+  | s::phi => (s, phi)
+  end.
+
+#[local] Arguments mk_ty /.
+
+Definition s_init : ty :=
+  mk_ty [arr' [hash; dollar] triangle].
+
+Definition s_star : ty := mk_ty [
+  arr' [arr' [bullet] star] star; 
+  arr' [arr' [isr] star] hash;
+  arr' [arr' [isl] hash; arr' [bullet] dollar] dollar].
+
+Definition s_0 : ty := mk_ty
+  [arr' [symbol 0] star; arr' [symbol 0] hash; arr' [symbol 1] dollar].
+
+Definition s_1 : ty := mk_ty [symbol 1].
+
+#[local] Notation rule := ((nat * nat) * (nat * nat))%type.
+
+Context (rs : list rule).
+
+Definition symbols :=
+  (flat_map (fun '((a,b),(c,d)) => [a; b; c; d]) rs) ++ [0; 1].
+
+Definition s_id_rules : list sty :=
+  map (fun (a : nat) => (arr' [bullet] (arr' [symbol a] (symbol a)))) symbols.
+
+Definition s_rule (r : rule) : ty :=
+  match r with
+  | ((x,y),(x',y')) => mk_ty (
+      (arr' [isl] (arr' [symbol x'] (symbol x))) ::
+      (arr' [isr] (arr' [symbol y'] (symbol y))) ::
+      s_id_rules)
+  end.
+
+Definition s_pos (i j : nat) : ty := if Nat.eqb i j then mk_ty [isl] else (if Nat.eqb i (S j) then mk_ty [isr] else mk_ty [bullet]).
+
+(*used for initialization, expansion, and termination*)
+Definition Γ_init : list ty := [s_init; s_star; s_0; s_1].
+
+Definition Γ_step : list ty := map s_rule rs.
+
+(*information on 'neighboring' environments*)
+Definition Γ_lr (bound : nat) (i : nat) : list ty := map (fun j => s_pos i j) (seq 0 bound).
+
+(*collection of all the above type environments*)
+Definition Γ_all (bound i : nat) :=
+  Γ_lr bound i ++ (Γ_init ++ Γ_step).
+
+(*
+Lemma In_nth_In t x (Gamma : list ty) :
+  In t (nth x Gamma []) ->
+  In (nth x Gamma []) Gamma.
+Proof.
+  elim: Gamma x. { by case. }
+  by move=> > IH [|x] => [|/IH] ?; [left|right].
+Qed.
+*)
+Lemma map_nth' {A B : Type} {f : A -> B} {l : list A} {d : B} {n : nat} (d' : A) :
+  n < length l -> nth n (map f l) d = f (nth n l d').
+Proof.
+elim: l n=> /=; first by lia.
+move=> ?? IH [|n] ?; first done.
+apply: IH. lia.
+Qed.
+
+Inductive Γ_all_spec (bound i x : nat) t : Prop :=
+  | Γ_all_lr_r : t = isr -> (forall i', nth_error (Γ_all bound i') x = Some (s_pos i' x)) -> i = S x -> x < bound -> Γ_all_spec bound i x t
+  | Γ_all_lr_l : t = isl -> (forall i', nth_error (Γ_all bound i') x = Some (s_pos i' x)) -> i = x -> x < bound -> Γ_all_spec bound i x t
+  | Γ_all_lr_bullet : t = bullet -> (forall i', nth_error (Γ_all bound i') x = Some (s_pos i' x)) -> i <> x -> i <> S x -> x < bound -> Γ_all_spec bound i x t
+  | Γ_all_init_init : t = (arr' [hash; dollar] triangle) -> (forall i', nth_error (Γ_all bound i') x = Some s_init) -> Γ_all_spec bound i x t
+  | Γ_all_init_star_star : t = (arr' [arr' [bullet] star] star) -> (forall i', nth_error (Γ_all bound i') x = Some s_star) -> Γ_all_spec bound i x t
+  | Γ_all_init_star_hash : t = (arr' [arr' [isr] star] hash) -> (forall i', nth_error (Γ_all bound i') x = Some s_star) -> Γ_all_spec bound i x t
+  | Γ_all_init_star_dollar : t = (arr' [arr' [isl] hash; arr' [bullet] dollar] dollar) -> (forall i', nth_error (Γ_all bound i') x = Some s_star) -> Γ_all_spec bound i x t
+  | Γ_all_init_0_star : t = (arr' [symbol 0] star) -> (forall i', nth_error (Γ_all bound i') x = Some s_0) -> Γ_all_spec bound i x t
+  | Γ_all_init_0_hash : t = (arr' [symbol 0] hash) -> (forall i', nth_error (Γ_all bound i') x = Some s_0) -> Γ_all_spec bound i x t
+  | Γ_all_init_0_dollar : t = (arr' [symbol 1] dollar) -> (forall i', nth_error (Γ_all bound i') x = Some s_0) -> Γ_all_spec bound i x t
+  | Γ_all_init_1 : t = (symbol 1) -> (forall i',nth_error (Γ_all bound i') x = Some s_1) -> Γ_all_spec bound i x t
+  | Γ_all_step_l a b a' b' : t = (arr' [isl] (arr' [symbol a'] (symbol a))) -> (forall i', nth_error (Γ_all bound i') x = Some (s_rule ((a, b), (a', b')))) -> In ((a, b), (a', b')) rs -> Γ_all_spec bound i x t
+  | Γ_all_step_r a b a' b' : t = (arr' [isr] (arr' [symbol b'] (symbol b))) -> (forall i', nth_error (Γ_all bound i') x = Some (s_rule ((a, b), (a', b')))) -> In ((a, b), (a', b')) rs -> Γ_all_spec bound i x t
+  | Γ_all_step_e a b a' b' e : t = (arr' [bullet] (arr' [symbol e] (symbol e))) -> (forall i', nth_error (Γ_all bound i') x = Some (s_rule ((a, b), (a', b')))) -> In ((a, b), (a', b')) rs -> In e symbols -> Γ_all_spec bound i x t.
+
+Lemma nth_Γ_common x bound i i' :
+  x >= length (Γ_lr bound i) ->
+  nth_error (Γ_all bound i') x = nth_error (Γ_all bound i) x.
+Proof.
+  move=> Hx. rewrite /Γ_all [LHS]nth_error_app2.
+  { move: Hx. by rewrite /Γ_lr !map_length !seq_length. }
+  rewrite [RHS]nth_error_app2; first done.
+  by rewrite /Γ_lr !map_length !seq_length.
+Qed.
+
+Lemma nth_error_seq start len n : n < len -> nth_error (seq start len) n = Some (start+n).
+Proof.
+  elim: len start n. { lia. }
+  move=> len IH start [|n] ?. { congr Some. lia. }
+  rewrite /= IH; [|congr Some]; lia.
+Qed.
+
+Lemma In_Γ_allE bound i x s phi t :
+  nth_error (Γ_all bound i) x = Some (s, phi) ->
+  In t (s::phi) ->
+  Γ_all_spec bound i x t.
+Proof.
+  have [|] : x < length (Γ_lr bound i) \/ x >= length (Γ_lr bound i) by lia.
+  { rewrite /Γ_lr map_length seq_length => Hx.
+    have H'x : forall i', nth_error (Γ_all bound i') x = Some (s_pos i' x).
+    { move=> i'. rewrite /Γ_all nth_error_app1. { by rewrite /Γ_lr map_length seq_length. }
+      by rewrite /Γ_lr nth_error_map nth_error_seq. }
+    rewrite H'x /s_pos. case Eix: (Nat.eqb i x) => /=.
+    { move=> [<- <-]. case; last done. move=> ?. move=> /Nat.eqb_eq in Eix. subst. by apply: Γ_all_lr_l. }
+    case E'ix: (Nat.eqb i (S x)).
+    { move=> [<- <-]. case; last done. move=> ?. move=> /Nat.eqb_eq in E'ix. subst. by apply: Γ_all_lr_r. }
+    move=> [<- <-]. case; last done. move=> <-. move=> /Nat.eqb_neq in Eix. move=> /Nat.eqb_neq in E'ix.
+    by apply: Γ_all_lr_bullet. }
+  rewrite /Γ_all. move=> /[dup] /nth_error_app2 + /nth_Γ_common.
+  rewrite /Γ_all. move=> ->. move: (x - _).
+  case. { move=> /= ? [<- <-]. by do 1 (case; [move=> <-; by eauto using Γ_all_spec, erefl with nocore|]). }
+  case. { move=> /= ? [<- <-]. by do 3 (case; [move=> <-; by eauto using Γ_all_spec, erefl with nocore|]). }
+  case. { move=> /= ? [<- <-]. by do 3 (case; [move=> <-; by eauto using Γ_all_spec, erefl with nocore|]). }
+  case. { move=> /= ? [<- <-]. by do 1 (case; [move=> <-; by eauto using Γ_all_spec, erefl with nocore|]). }
+  move=> x' /=.
+  rewrite /Γ_step nth_error_map. move E: (nth_error rs x') => [[[? ?][? ?]]|]; last done.
+  move=> /(@nth_error_In rule) in E.
+  move=> ? [<- <-] /=.
+  do 2 (case; [move=> <-; by eauto using Γ_all_spec, erefl with nocore|]).
+  move=> /in_map_iff [?] [<-]. by eauto using Γ_all_spec, erefl with nocore.
+Qed.
+
+(*only s_rule can be used deriving a type with two parameters for a normal form*)
+Lemma two_params_rule (bound i: nat) N phi psi (s1 s2 t : sty) :
+  head_form N ->
+  type_assignment (Γ_all bound i) N (arr s1 phi (arr s2 psi t)) ->
+  (exists x (e : nat), N = var x /\ t = symbol e).
+Proof.
+  move=> H. elim: H s1 phi s2 psi t.
+  { move=> x > /type_assignmentE [] > /In_Γ_allE /[apply].
+    move=> [] // > [] *; subst; by eexists _, _. }
+  move=> > ? IH ? > /type_assignmentE [] > /IH.
+  firstorder done.
+Qed.
+
+Lemma nf_hf_atom Gamma N a :
+  normal_form N ->
+  type_assignment Gamma N (atom a) ->
+  head_form N.
+Proof.
+  case; [done|]. by move=> ?? /type_assignmentE.
+Qed.
+
+(*if triangle is inhabited in (Γ_init ++ Γ_step rs), then hash, dollar is inhabited in (Γ_all rs 0 0)*)
+Lemma soundness_init (N : tm) :
+  head_form N ->
+  type_assignment (Γ_init ++ Γ_step) N triangle ->
+  exists (N' : tm), head_form N' /\
+  type_assignment (Γ_all 0 0) N' hash /\
+  type_assignment (Γ_all 0 1) N' dollar.
+Proof.
+  case.
+  { move=> x /type_assignmentE [>] /(In_Γ_allE 0 0) /[apply]. by case. }
+  move=> ? N' []; first last.
+  { move=> > /two_params_rule H ??.
+    move=> /type_assignmentE [>] /type_assignmentE [>].
+    by move=> /(H 0 0) [?] [?] []. }
+  move=> ?? /type_assignmentE [>] /type_assignmentE [>] /(In_Γ_allE 0 0) /[apply].
+  case=> //.
+  move=> [-> ->] ? ? /Forall_cons_iff [? _].
+  exists N'. split; last done.
+  apply: nf_hf_atom; by eassumption.
+Qed.
+
+(* induction/recursion principle wrt. a decreasing measure f *)
+(* example: elim /(measure_rect length) : l. *)
+Lemma measure_rect {X : Type} (f : X -> nat) (P : X -> Type) : 
+(forall x, (forall y, f y < f x -> P y) -> P x) -> forall (x : X), P x.
+Proof.
+  exact: (well_founded_induction_type (Wf_nat.well_founded_lt_compat X f _ (fun _ _ => id)) P).
+Qed.
+
+Lemma Γ_lr_bound_S bound : Γ_lr bound (S bound) = map (fun=> (bullet, [])) (seq 0 bound).
+Proof.
+  apply: map_ext_in => j /in_seq ?. rewrite /s_pos.
+  have /Nat.eqb_neq -> : S bound <> j by lia.
+  by have /Nat.eqb_neq -> : S bound <> S j by lia.
+Qed.
+
+(*if stars, hash, dollar is inhabited in (Γ_all rs bound [0 .. 1+bound]), then 0 is inhabited in (Γ_all rs bound [0 .. bound'])*)
+Lemma soundness_expand (bound : nat) (N : tm) :
+  head_form N ->
+  Forall (fun Γi => type_assignment Γi N star) (map (Γ_all bound) (seq 1 bound)) ->
+  type_assignment (Γ_all bound 0) N hash ->
+  type_assignment (Γ_all bound (1+bound)) N dollar ->
+  exists bound' N',
+    head_form N' /\
+    Forall (fun Γi => type_assignment Γi N' (symbol 0)) (map (Γ_all bound') (seq 0 (1+bound'))).
+Proof.
+  elim /(measure_rect tm_size): N bound.
+  move=> ? + bound Hx. case: Hx.
+  { move=> ? IH ? /type_assignmentE [>] /In_Γ_allE /[apply]. by case. }
+  move=> M N []; first last.
+  { move=> > /two_params_rule H ???? /type_assignmentE [>] /type_assignmentE [>].
+    by move=> /H [?] [?] []. }
+  move=> ? H0N IH IH' /type_assignmentE [>] /type_assignmentE [>].
+  move=> /In_Γ_allE /[apply]. case=> //.
+  - move=> [-> ->] Hx H1N _.
+    move: H0N IH IH' H1N => [].
+    { move=> ? [].
+      - move=> ??? /type_assignmentE [>] /In_Γ_allE /[apply]. by case.
+      - by move=> > /two_params_rule H ??? /type_assignmentE [>] /H [?] [?] []. }
+    move=> N' H0N' IH IH' /type_assignmentE H1N'.
+    move=> /type_assignmentE [>] /type_assignmentE [>].
+    rewrite Hx=> - [<- <-]. case; [done|case;[done|case;[|done]]].
+    move=> [<- <-]/type_assignmentE H2N' /Forall_cons_iff [/type_assignmentE H3N' _].
+    apply: (IH N' _ (S bound)).
+    + move=> /=. lia.
+    + by apply: nf_hf_atom; eassumption.
+    + move=> /=. constructor.
+      { move: H1N'. by rewrite /Γ_all /= -seq_shift map_map. }
+      move: IH'. rewrite -!seq_shift !map_map.
+      move=> /Forall_map IH'. apply /Forall_map. apply: Forall_impl IH'.
+      move=> ? /type_assignmentE [>] /type_assignmentE [>].
+      rewrite Hx=> - [<- <-]. case; [|case;[done|by case]].
+      move=> [<- <-] /type_assignmentE + _.
+      by rewrite /Γ_all /= -seq_shift map_map.
+    + move: H2N'. congr type_assignment.
+      rewrite /Γ_all /=. congr cons. congr List.app.
+      rewrite -seq_shift map_map. apply: map_ext_in => j /in_seq ?. rewrite /s_pos.
+      have /Nat.eqb_neq -> : S bound <> j by lia.
+      by have /Nat.eqb_neq -> : S bound <> S j by lia.
+    + move: H3N'. by rewrite /Γ_all /= -seq_shift map_map.
+  - move=> [-> ->] Hx ? _ /type_assignmentE [>] /type_assignmentE [>].
+    rewrite Hx=> - [<- <-]. case; [done|case;[done|case;[|done]]].
+    move=> [<- <-] ? _.
+    exists bound, N. split. { by apply: nf_hf_atom; eassumption. }
+    move=> /=. constructor; [done|].
+    apply /Forall_forall => ? /[dup] /in_map_iff [?] [<-] ?.
+    move: IH' => /Forall_forall /[apply].
+    move=> /type_assignmentE [>] /type_assignmentE [>].
+    rewrite Hx=> - [<- <-]. case; [|case;[done|by case]].
+    by move=> [<- <-].
+Qed.
+
+Lemma Forall_nth_const v :
+  Forall (fun i => nth i v 0 = 1) (seq 0 (length v)) ->
+  v = repeat 1 (length v).
+Proof.
+  elim: v; first done.
+  move=> ? v IH /= /Forall_cons_iff [->].
+  by rewrite -seq_shift Forall_map => /IH <-.
+Qed.
+
+Lemma s_rule_spec bound x s1 phi s2 psi a N :
+  type_assignment (Γ_all bound bound) (var x) (arr s1 phi (arr s2 psi (symbol a))) ->
+  normal_form N ->
+  type_assignment (Γ_all bound bound) N s1 ->
+  (exists r, In r rs /\ (forall i', nth_error (Γ_all bound i') x = Some (s_rule r))) /\
+  exists y, N = var y /\ y < bound /\ (forall i', nth_error (Γ_all bound i') y = Some (s_pos i' y)).
+Proof.
+  move=> /type_assignmentE [>] /In_Γ_allE /[apply] Hx HN Hs1. split.
+  { by case: Hx => // *; eexists; split; eassumption. }
+  have {}HN : head_form N.
+  { case: HN Hs1; first done.
+    move=> ? ?. move: Hx.
+    by case=> // > [?????] _ _ => [| |_]; subst => /type_assignmentE. }
+  case: HN Hs1.
+  { move=> y Hy. exists y. split; first done.
+    case: Hx Hy => // > [-> ????] _ _ => [| |_].
+    all: by move=> /type_assignmentE [>] /In_Γ_allE /[apply] - []. }
+  move=> > [].
+  { move=> ??. move: Hx.
+    case=> // > [-> ????] _ _ => [| |_].
+    all: move=> /type_assignmentE [>] /type_assignmentE [>].
+    all: by move=> /In_Γ_allE /[apply] - []. }
+  move=> > /two_params_rule H ??. move: Hx.
+  case=> // > [-> ????] _ _ => [| |_].
+  all: move=> /type_assignmentE [>] /type_assignmentE [>].
+  all: by move=> /H [?] [?] [].
+Qed.
+
+Inductive In_s_rule (t : sty) (a b a' b': nat) : Prop :=
+  | In_s_rule_a_a' : t = arr' [isl] (arr' [symbol a'] (symbol a)) -> In_s_rule t a b a' b'
+  | In_s_rule_b_b' : t = arr' [isr] (arr' [symbol b'] (symbol b)) -> In_s_rule t a b a' b'
+  | In_s_rule_id e : t = arr' [bullet] (arr' [symbol e] (symbol e)) -> In e symbols -> In_s_rule t a b a' b'.
+
+Lemma In_s_rule_spec t a b a' b' :
+  let '(s, phi) := s_rule (a, b, (a', b')) in
+  In t (s::phi) ->
+  In_s_rule t a b a' b'.
+Proof.
+  move=> /= [|[|/in_map_iff [?] []]].
+  all: by eauto using In_s_rule, esym with nocore.
+Qed.
+
+(*if [a_0 .. a_bound] is inhabited in (Γ_all bound [0 .. bound], then a_0..a_bound rewrites to 1..1 *)
+Lemma soundness_step (bound : nat) (N : tm) (v : list nat) :
+  head_form N ->
+  length v = bound + 1 ->
+  Forall (fun i => type_assignment (Γ_all bound i) N (symbol (nth i v 0))) (seq 0 (bound + 1)) ->
+  multi_step rs v (repeat 1 (bound + 1)).
+Proof.
+  elim /(measure_rect tm_size): N v.
+  move=> N IH v H0N Hv /[dup] H'v.
+  rewrite seq_app /= => /Forall_app [_] /Forall_cons_iff [+ _].
+  case: H0N IH H'v.
+  { move=> ?? H /type_assignmentE [>] /In_Γ_allE /[apply] - [] // ? Hx.
+    rewrite (Forall_nth_const v); rewrite Hv; last by apply: rt_refl.
+    apply: Forall_impl H => ? /type_assignmentE [>].
+    rewrite Hx=> - [<- <-]. by case; case. }
+  move=> ? N1 [].
+  { by move=> ???? /type_assignmentE [>] /type_assignmentE [>] /In_Γ_allE /[apply] - []. }
+  move=> ? N2 /two_params_rule H HN2 HN1 IH IH'.
+  move=> /type_assignmentE [>] /type_assignmentE [>] /[dup] H' /H{H}.
+  move=> [?] [?] [? _]. subst.
+  move: (H') HN2 => /s_rule_spec /[apply] /[apply].
+  move=> [[[[a0 b0][a1 b1]]]] [Hr] Hx [y] [?] [H1y H2y] H'N2 H1N1 H2N1. subst.
+  have Ha0 : nth_error v y = Some a0.
+  { have : In y (seq 0 (bound + 1)) by apply /in_seq; lia.
+    move: IH' => /Forall_forall /[apply].
+    move=> /type_assignmentE [>] /type_assignmentE [>] /type_assignmentE [>].
+    rewrite Hx=> - [<- <-].
+    move=> H'' /type_assignmentE [>].
+    rewrite H2y /s_pos Nat.eqb_refl => - [<- <-]. case; last done.
+    move=> ?. subst. move: H'' => /In_s_rule_spec [] //.
+    move=> [] *. subst. apply: nth_error_nth'. lia. }
+  have Hb0 : nth_error v (S y) = Some b0.
+  { have : In (S y) (seq 0 (bound + 1)) by apply /in_seq; lia.
+    move: IH' => /Forall_forall /[apply].
+    move=> /type_assignmentE [>] /type_assignmentE [>] /type_assignmentE [>].
+    rewrite Hx=> - [<- <-].
+    move=> H'' /type_assignmentE [>].
+    rewrite H2y /s_pos Nat.eqb_refl.
+    have /Nat.eqb_neq -> : S y <> y by lia.
+    move=> [<- <-]. case; last done. move=> ?. subst.
+    move: H'' => /In_s_rule_spec [] //.
+    move=> [] *. subst. apply: nth_error_nth'. lia. }
+  move: Hr Ha0 Hb0 => /step_spec /[apply] /[apply] ?.
+  apply: rt_trans. { apply: rt_step. eassumption. }
+  apply: (IH N1).
+  - move=> /=. lia.
+  - move: H' H1N1 => /type_assignmentE [>] /In_Γ_allE /[apply].
+    case=> // > [?????] _ _ => [| |_]; subst.
+    all: move=> /nf_hf_atom; by apply.
+  - by rewrite map_length seq_length.
+  - apply /Forall_forall => i /[dup] /in_seq [_ ?].
+    move: IH' => /Forall_forall /[apply].
+    move=> /type_assignmentE [>] /type_assignmentE [>] /type_assignmentE [>].
+    rewrite Hx=> - [<- <-].
+    move=> H'x /type_assignmentE [>].
+    rewrite H2y /s_pos.
+    case E1iy: (Nat.eqb i y).
+    { move=> [<- <-]. case; last done. move=> ? _. subst.
+      move: H'x => /In_s_rule_spec [] //.
+      move=> [? -> ??] + _. congr type_assignment. congr symbol.
+      rewrite (map_nth' 0). { by rewrite seq_length Hv. }
+      rewrite seq_nth /= ?E1iy; lia. }
+    case E2iy: (Nat.eqb i (S y)).
+    { move=> [<- <-]. case; last done. move=> ? _. subst.
+      move: H'x => /In_s_rule_spec [] //.
+      move=> [? -> ??] + _. congr type_assignment. congr symbol.
+      rewrite (map_nth' 0). { by rewrite seq_length Hv. }
+      rewrite seq_nth /= ?E1iy ?E2iy; lia. }
+    move=> [<- <-]. case; last done. move=> ? _. subst.
+    move: H'x => /In_s_rule_spec [] //.
+    move=> e [? -> ??] ? + _. congr type_assignment. congr symbol.
+    rewrite (map_nth' 0). { by rewrite seq_length Hv. }
+    rewrite seq_nth /= ?E1iy ?E2iy; lia.
+Qed.
+
+(*if triangle is inhabited in (Γ_init ++ Γ_step rs), then 0..0 rewrites to 1..1*)
+Theorem soundness N :
+  normal_form N ->
+  type_assignment (Γ_init ++ Γ_step) N triangle ->
+  exists (m : nat), multi_step rs (repeat 0 (1+m)) (repeat 1 (1+m)).
+Proof.
+  move=> /nf_hf_atom + /[dup] => /[apply].
+  move=> /soundness_init /[apply] - [N'] [] + [].
+  move=> /(soundness_expand 0) /[apply] /[apply] => /(_ (Forall_nil _)).
+  move=> [bound] [N''] [] /soundness_step H H'.
+  exists bound. move: H'. have -> : 1 + bound = bound + 1 by lia.
+  move=> H'. apply: H. { by rewrite repeat_length. }
+  move: H' => /Forall_map. apply: Forall_impl => i.
+  by rewrite nth_repeat.
+Qed.
+
+(* COMPLETENESS *)
+
+(*hash, dollar is inhabited in Γ_all rs 0 [0, 1], then triangle is inhabited in (Γ_init ++ Γ_step rs)*)
+Lemma completeness_init N :
+  head_form N ->
+  type_assignment (Γ_all 0 0) N hash ->
+  type_assignment (Γ_all 0 1) N dollar ->
+  exists N', normal_form N' /\ type_assignment (Γ_init ++ Γ_step) N' triangle.
+Proof.
+  move=> ???.
+  exists (app (var 0) N). split. { by do ? constructor. }
+  apply: type_assignment_app.
+  - constructor. by left.
+  - by do ? constructor.
+Qed.
+
+Lemma In_Γ_all_skip_lr t bound n i :
+  In t (nth n ((Γ_init ++ Γ_step)) []) ->
+  In t (nth (bound + n) (Γ_all bound i) []).
+Proof.
+  rewrite /Γ_all /Γ_lr [nth (bound + n) _ _](@app_nth2 ty) map_length seq_length. { lia. }
+  congr In. congr nth. lia.
+Qed.
+
+(*if stars, hash, dollar is inhabited in Γ_all rs bound [0..bound-1, bound, bound+1], then hash, dollar is inhabited in Γ_all rs 0 [0, 1]*)
+Lemma completeness_expand bound N :
+  head_form N ->
+  Forall (fun (i : nat) => type_assignment (Γ_all bound i) N star) (seq 1 bound) ->
+  type_assignment (Γ_all bound 0) N hash ->
+  type_assignment (Γ_all bound (1 + bound)) N dollar ->
+  exists N', 
+    head_form N' /\
+    type_assignment (Γ_all 0 0) N' hash /\ 
+    type_assignment (Γ_all 0 1) N' dollar.
+Proof.
+  elim: bound N. { move=> *. eexists. by split; [eassumption|]. }
+  move=> bound IH N HN H1N H2N H3N.
+  apply: (IH (app (var (bound + 1)) (lam N))).
+  - by eauto using head_form, normal_form with nocore.
+  - move: H1N => /= /Forall_cons_iff [_].
+    rewrite -!seq_shift !map_map => /Forall_map H'N.
+    apply /Forall_map. apply: Forall_impl H'N => ? H'N.
+    apply: type_assignment_app.
+    + constructor. apply: In_Γ_all_skip_lr. by left.
+    + do ? constructor. move: H'N. by rewrite /Γ_all /= -seq_shift map_map.
+  - apply: type_assignment_app.
+    + constructor. apply: In_Γ_all_skip_lr. right. by left.
+    + do ? constructor. move: H1N => /Forall_cons_iff [+ _].
+      by rewrite /Γ_all /= -seq_shift map_map.
+  - apply: type_assignment_app.
+    + constructor. apply: In_Γ_all_skip_lr. right. right. by left.
+    + do ? constructor.
+      * move: H2N. by rewrite /Γ_all /= -seq_shift map_map Γ_lr_bound_S.
+      * move: H3N. by rewrite /Γ_all /= -seq_shift map_map.
+Qed.
+
+Lemma completeness_0 bound N :
+  head_form N ->
+  Forall (fun (i : nat) => type_assignment (Γ_all bound i) N (symbol 0)) (seq 0 (S bound)) ->
+  type_assignment (Γ_all bound (1 + bound)) N (symbol 1) ->
+  exists N', 
+    head_form N' /\
+    Forall (fun (i : nat) => type_assignment (Γ_all bound i) N' star) (seq 1 bound) /\
+    type_assignment (Γ_all bound 0) N' hash /\
+    type_assignment (Γ_all bound (1 + bound)) N' dollar.
+Proof.
+  move=> ? /= /Forall_cons_iff [H1N H2N] H3N.
+  exists (app (var (bound + 2)) N). do ? split.
+  - by eauto using head_form, normal_form with nocore.
+  - apply: Forall_impl H2N => ? ?. apply: type_assignment_app.
+    + constructor. apply: In_Γ_all_skip_lr. by left.
+    + by do ? constructor.
+  - apply: type_assignment_app.
+    + constructor. apply: In_Γ_all_skip_lr. right. by left.
+    + by do ? constructor.
+  - apply: type_assignment_app.
+    + constructor. apply: In_Γ_all_skip_lr. right. right. by left.
+    + by do ? constructor.
+Qed.
+
+Lemma In_s_id_rulesI c a b a' b' :
+  In c symbols -> In (arr [bullet] (arr [symbol c] (symbol c))) (s_rule (a, b, (a', b'))).
+Proof. move=> ?. do 2 right. apply /in_map_iff. by exists c. Qed.
+
+Lemma nth_Γ_lr i j bound : j < bound -> nth j (Γ_all bound i) [] = s_pos i j.
+Proof.
+  move=> ?. rewrite /Γ_all /Γ_lr (@app_nth1 ty). { by rewrite map_length seq_length. }
+  rewrite (map_nth' 0). { by rewrite seq_length. }
+  by rewrite seq_nth.
+Qed.
+
+Lemma completeness_step (bound : nat) (N : tm) (v w : list nat) :
+  step rs v w ->
+  (forall i, In (nth i v 0) symbols) ->
+  head_form N ->
+  length v = bound + 1 ->
+  type_assignment (Γ_all bound (1 + bound)) N (symbol 1) ->
+  Forall (fun i => type_assignment (Γ_all bound i) N (symbol (nth i w 0))) (seq 0 (bound + 1)) ->
+  exists N',
+    head_form N' /\
+    type_assignment (Γ_all bound (1 + bound)) N' (symbol 1) /\
+    Forall (fun i => type_assignment (Γ_all bound i) N' (symbol (nth i v 0))) (seq 0 (bound + 1)).  
+Proof.
+  case=> u1 u2 a0 b0 a1 b1. rewrite !app_length /= => + ??? H1N H2N.
+  move=> /(@In_split rule) [rs1] [rs2] Hrs.
+  have ? : length u1 < bound by lia.
+  pose x := bound + (length Γ_init + length rs1).
+  have Hx : forall i, nth x (Γ_all bound i) [] = s_rule ((a0, b0), (a1, b1)).
+  { move=> i. rewrite /x /Γ_all /Γ_step Hrs map_app (@app_nth2 ty) map_length seq_length. { lia. }
+    have -> /= : forall n, bound + n - bound = n by lia.
+    by rewrite (@app_nth2 ty) map_length ?Nat.sub_diag. }
+  exists (app (app (var x) (var (length u1))) N). do ? split.
+  - by eauto using head_form, normal_form with nocore.
+  - apply: type_assignment_app; [apply: type_assignment_app|].
+    + constructor. rewrite Hx. apply: In_s_id_rulesI. apply /in_app_iff. do 2 right. by left.
+    + do ? constructor. rewrite nth_Γ_lr. { done. }
+      rewrite /s_pos.
+      have /Nat.eqb_neq -> : S bound <> 0 + length u1 by lia.
+      have /Nat.eqb_neq -> : S bound <> S (0 + length u1) by lia.
+      by left.
+    + by do ? constructor.
+  - apply /Forall_forall => i /[dup] /in_seq [_ ?].
+    move: H2N => /Forall_forall /[apply].
+    have [Hi|[Hi|Hi]] : (i < length u1 \/ i >= length u1 + 2) \/ i = length u1 \/ i = S (length u1) by lia.
+    + move=> H'N. apply: type_assignment_app; [apply: type_assignment_app|].
+      * constructor. rewrite Hx. by apply: In_s_id_rulesI.
+      * do ? constructor. rewrite nth_Γ_lr. { done. }
+        rewrite /s_pos.
+        have /Nat.eqb_neq -> : i <> length u1 by lia.
+        have /Nat.eqb_neq -> : i <> S (length u1) by lia.
+        by left.
+      * do ? constructor. move: H'N. congr type_assignment. congr symbol.
+        case: Hi => ?. { by do 2 (rewrite (@app_nth1 nat); first done). }
+        do 2 (rewrite (@app_nth2 nat); first lia).
+        by have ->: i - length u1 = S (S (i - length u1 - 2)) by lia.
+    + rewrite Hi (@app_nth2 nat). { done. }
+      rewrite (@app_nth2 nat) ?Nat.sub_diag. { done. }
+      move=> /= H'N. apply: type_assignment_app; [apply: type_assignment_app|].
+      * constructor. rewrite Hx. by left.
+      * do ? constructor. rewrite nth_Γ_lr. { done. }
+        rewrite /s_pos Nat.eqb_refl. by left.
+      * by do ? constructor.
+    + rewrite Hi (@app_nth2 nat). { lia. }
+      rewrite (@app_nth2 nat). { lia. }
+      have -> : S (length u1) - length u1 = 1 by lia.
+      move=> /= H'N. apply: type_assignment_app; [apply: type_assignment_app|].
+      * constructor. rewrite Hx. right. by left.
+      * do ? constructor. rewrite nth_Γ_lr. { done. }
+        rewrite /s_pos Nat.eqb_refl.
+        have /Nat.eqb_neq -> : S (length u1) <> length u1 by lia.
+        by left.
+      * by do ? constructor.
+Qed.
+
+Lemma step_symbols v w :
+  step rs v w ->
+  (forall i : nat, In (nth i v 0) symbols) ->
+  (forall i : nat, In (nth i w 0) symbols).
+Proof.
+  case=> u1 u2 > Hr H i. move: (H i).
+  have [Hi|[->|[->|Hi]]] : i < length u1 \/ i = length u1 \/ i = S (length u1) \/ i >= length u1 + 2 by lia.
+  - by rewrite !(@app_nth1 nat).
+  - move=> _. rewrite (@app_nth2 nat) ?Nat.sub_diag. { done. }
+    apply /in_app_iff. left. apply /in_flat_map.
+    eexists. split; [eassumption|].
+    move=> /=. tauto.
+  - move=> _. rewrite (@app_nth2 nat). { lia. }
+    have -> : S (length u1) - length u1 = 1 by lia.
+    apply /in_app_iff. left. apply /in_flat_map.
+    eexists. split; [eassumption|].
+    move=> /=. tauto.
+  - rewrite (@app_nth2 nat). { lia. }
+    rewrite (@app_nth2 nat). { lia. }
+    by have -> : i - length u1 = S (S (i - length u1 - 2)) by lia.
+Qed.
+
+Lemma completeness_star (bound : nat) (N : tm) (v : list nat) :
+  multi_step rs v (repeat 1 (1+bound)) ->
+  (forall i, In (nth i v 0) symbols) ->
+  head_form N ->
+  length v = bound + 1 ->
+  type_assignment (Γ_all bound (1 + bound)) N (symbol 1) ->
+  Forall (fun i => type_assignment (Γ_all bound i) N (symbol 1)) (seq 0 (bound + 1)) ->
+  exists N',
+    head_form N' /\
+    type_assignment (Γ_all bound (1 + bound)) N' (symbol 1) /\
+    Forall (fun i => type_assignment (Γ_all bound i) N' (symbol (nth i v 0))) (seq 0 (bound + 1)).  
+Proof.
+  move=> /clos_rt_rt1n_iff. move E: (repeat 1 (1+bound)) => w Hvw.
+  elim: Hvw E N; clear v w.
+  { move=> ? <- N ??? HN. exists N. split; [done|split;[done|]].
+    apply: Forall_In_impl H => i /in_seq ?. congr type_assignment. congr symbol.
+    rewrite (nth_indep _ 0 1). { rewrite repeat_length. lia. }
+    by rewrite nth_repeat. }
+  move=> v u w /[dup] /step_length_eq Hvu /[dup] /step_symbols H'vu.
+  move=> /completeness_step H _ /[apply] + N /[dup] Hv /H'vu ++ /[dup] H'v.
+  rewrite Hvu. do 5 move=> /[apply]. move=> [N'] [?] [? ?]. by apply: H; eassumption.
+Qed.
+
+Lemma completeness (m : nat) :
+  multi_step rs (repeat 0 (1+m)) (repeat 1 (1+m)) ->
+  exists N, normal_form N /\ type_assignment (Γ_init ++ Γ_step) N triangle.
+Proof.
+  move=> /completeness_star => /(_ (var (m + 3))).
+  apply: unnest. { move=> ?. rewrite nth_repeat. apply /in_app_iff. right. by left. }
+  apply: unnest. { by constructor. }
+  apply: unnest. { rewrite repeat_length. lia. }
+  apply: unnest. { constructor. apply: In_Γ_all_skip_lr. by left. }
+  apply: unnest. { apply /Forall_forall => ??. constructor. apply: In_Γ_all_skip_lr. by left. }
+  move=> [N'] [+] [+] HN' => /completeness_0 /[apply].
+  apply: unnest. { move: HN'. have -> : m + 1 = S m by lia. apply: Forall_impl => ?. by rewrite nth_repeat. }
+  move=> [N''] [+] [+] [+] => /completeness_expand /[apply] /[apply] /[apply].
+  move=> [N'''] [?] [?] ?. by apply: completeness_init; eassumption.
+Qed.
+
+Print Assumptions completeness.
+Print Assumptions soundness.
